TabularTypeInterpreter/List.lean
@@ -1,33 +1,35 @@
+import Mathlib.Data.List.Basic
+import TabularTypeInterpreter.Range
+
 namespace List
-
--- TODO better get some sane names for these
-theorem whateverL1 : l1.length = l2.length -> map (f ∘ Prod.fst) (zip l1 l2) = map f l1 := sorry
-theorem whateverL2 : l1.length = l2.length -> map (f ∘ Prod.snd) (zip l1 l2) = map f l2 := sorry
-theorem whateverflat : (map (fun x => [f x]) l).flatten = map f l := sorry
-
-theorem zip_member : (a,b) ∈ zip l1 l2 → a ∈ l1 ∧ b ∈ l2 := by
-  intro h
-  induction l1 generalizing l2 <;> (try simp_all; done)
-  . case cons _ _ hd1 tl1 ih1 =>
-    induction l2
-    . case nil => simp_all
-    . case cons hd2 tl2 ih2 =>
-      simp_all
-      cases h
-      . case inl => simp_all
-      . case inr H =>
-        have H' := ih1 H
-        simp_all
-
-theorem zip_member_map_same : (a,b) ∈ zip (map f l) (map g l) -> ∃ c, c ∈ l ∧ a = f c ∧ b = g c := by
-  induction l
-  . case nil => simp_all
-  . case cons =>
-    simp_all
-    intro h
-    cases h <;> simp_all
 
 def combinations {α : Type} (l : List α) :  List (List α)  :=
   l.foldl (fun acc a => acc ++ acc.map (fun l => a :: l)) [nil]
+
+def toFn {α: Type} (l: List α) (default: α) (n: Nat): α :=
+  if h: n < l.length then
+    l.get (.mk n h)
+  else
+    default -- it doesn't really matter what we return here
+
+def toFn_spec {d: α} {l: List α} i (le: i < l.length): l.toFn d i = l[i] := by simp_all [toFn]
+
+theorem toFn_spec' {d: α} {l: List α}: [0:l.length].map (l.toFn d) = l := by
+  induction l using List.reverseRecOn
+  . case nil => simp_all [Std.Range.toList]
+  . case append_singleton xs x ih =>
+    simp_all [Std.Range.map]
+    rw [<- Std.Range.toList_append (m := xs.length)] <;> simp_all
+    have aux : ∀α (a b c d: List α), a = b → c = d → a ++ c = b ++ d := by simp
+    apply aux
+    . rw (occs := .pos [3]) [<- ih]
+      apply List.map_congr_left
+      intro a In
+      apply Std.Range.mem_toList_le at In
+      have In' : a < xs.length + 1 := by simp_all [Nat.lt_add_right]
+      simp_all [toFn]
+      simp_all [List.getElem_append]
+      simp
+    . simp [Std.Range.toList, toFn]
 
 end List
