TabularTypeInterpreter/Range.lean
@@ -1,0 +1,47 @@
+import Lott.Data.Range
+
+namespace Std.Range
+
+private
+theorem mem_of_mem_toList {m n i: Nat} (mem: i ∈ [m:n].toList): i ∈ [m:n] := by
+  have H := @mem_of_mem_map (f:=id)
+  simp_all
+
+private
+theorem mem_toList_of_mem {m n i: Nat} (mem: i ∈ [m:n]): i ∈ [m:n].toList := by
+  have H := @mem_map_of_mem (f:=id)
+  simp_all
+
+theorem mem_toList_le {m} n {h: m <= n} : ∀i ∈ [m:n].toList, i < n := by
+  intros i In
+  induction n
+  . case zero => simp_all [Std.Range.toList]
+  . case succ n ih =>
+    rw [<- Std.Range.toList_append (m := n) (by
+      cases h
+      . case refl =>
+        simp [Std.Range.toList] at In
+      . case step => simp_all
+    ) (by
+      cases h
+      . case refl =>
+        simp [Std.Range.toList] at In
+      . case step => simp_all
+    )] at In
+    simp_all
+    cases In
+    .case inl In =>
+      cases h
+      . case refl =>
+        exfalso
+        unfold Std.Range.toList at In
+        simp at In
+        cases In; case intro h _ =>
+        exact Nat.lt_irrefl _ (Nat.lt_of_add_right_lt h)
+      . case step =>
+        simp_all [Nat.lt_add_right]
+    . case inr h =>
+      simp [Std.Range.toList] at h
+      simp_all
+
+end Std.Range
